improve cameligo extract

extraction/theories/CameLIGOExtract.v
@@ -22,7 +22,7 @@ From Coq Require Import List Ascii String.
 Local Open Scope string_scope.
 
 From MetaCoq.Template Require Import All.
-
+From MetaCoq.PCUIC Require PCUICAst PCUICTyping.
 
 Definition to_constant_decl (gd : option T.global_decl) :=
   match gd with
@@ -48,32 +48,85 @@ Arguments lmd_receive {_ _ _ _ _ _}.
 Arguments lmd_receive_prelude {_ _ _ _ _ _}.
 Arguments lmd_entry_point {_ _ _ _ _ _}.
 
-Definition printCameLIGODefs (prefix : string) (Σ : global_env)
+Definition cameligo_args :=
+  {| optimize_prop_discr := true;
+     transforms := [Optimize.dearg_transform
+                      true
+                      false (* cannot have aprtially applied ctors *)
+                      true
+                      true
+                      true] |}.
+
+Import PCUICAst PCUICTyping.
+Definition annot_extract_env_cameligo
+           (Σ : PCUICAst.global_env) 
+           (wfΣ : ∥wf Σ∥)
+           (include : KernameSet.t)
+           (ignore : kername -> bool) : option (∑ Σ, env_annots box_type Σ).
+Proof.
+  unshelve epose proof (annot_extract_pcuic_env cameligo_args Σ wfΣ include ignore _).
+  - constructor; [|constructor].
+    apply annot_dearg_transform.
+  - destruct extract_pcuic_env; [|exact None].
+    exact (Some (t; X)).
+Defined.
+
+
+Definition annot_extract_template_env_specalize
+           (e : TemplateEnvironment.global_env)
+           (seeds : KernameSet.t)
+           (ignore : kername -> bool) : result (∑ e, env_annots box_type e) string :=
+  let e := SafeTemplateChecker.fix_global_env_universes e in
+  let e := T2P.trans_global_decls e in
+  e <- specialize_ChainBase_env e ;;
+  wfe <-check_wf_env_func extract_within_coq e;;
+  match annot_extract_env_cameligo e wfe seeds ignore with
+  | Some s => Ok s
+  | None => Err "failed internally in annot_extract_template_env_specalize"
+  end. 
+
+Definition printCameLIGODefs (prefix : string) (Σ : TemplateEnvironment.global_env)
            (TT : MyEnv.env string)
-           (temp_env : extract_template_env_params)
            (ignore : list kername)
            (build_call_ctx : string)
            (init_prelude : string)
+           (receive_prelude : string)
            (init : kername)
            (receive : kername)
   : string + string :=
   let seeds := KernameSet.union (KernameSet.singleton init) (KernameSet.singleton receive) in
-  match annot_extract_template_env_specalize temp_env Σ seeds (fun k => List.existsb (eq_kername k) ignore) with
+  match annot_extract_template_env_specalize Σ seeds (fun k => List.existsb (eq_kername k) ignore) with
   (* match extract_template_env_within_coq Σ seeds (fun k => List.existsb (eq_kername k) ignore) with *)
   | Ok (eΣ; annots) => 
     (* dependencies should be printed before the dependent definitions *)
     let ldef_list := List.rev (print_global_env prefix TT eΣ annots) in
     (* filtering empty strings corresponding to the ignored definitions *)
-    let ldef_list := filter (negb ∘ (String.eqb "") ∘ snd) ldef_list in
+    let not_empty_str := (negb ∘ (String.eqb "") ∘ snd) in
+    
+    let ldef_ty_list := ldef_list 
+                          |> filter (fun d => match d with TyDecl _ => true | _ => false end)
+                          |> map (fun d => match d with ConstDecl d' => d' | TyDecl d' => d' end)
+                          |> filter not_empty_str in
+    let ldef_const_list := ldef_list 
+                            |> filter (fun d => match d with ConstDecl _ => true | _ => false end)
+                            |> map (fun d => match d with ConstDecl d' => d' | TyDecl d' => d' end)
+                            |> filter not_empty_str in
+    (* look for init function *)
     match bigprod_find (fun '(k, _, _) _ => eq_kername k init) annots with
     | Some ((_, ExAst.ConstantDecl init_cst); annots) =>
       match print_init prefix TT build_call_ctx init_prelude eΣ init_cst annots with
       | Some init_code =>
         (* filtering out the definition of [init] and projecting the code *)
-        let defs :=
-            map snd (filter (negb ∘ (eq_kername init) ∘ fst) ldef_list) in
-        let res :=
-            concat (nl ++ nl) (defs ++[ init_code ]) %list in
+        (* and place receive_prelude after type decls and before constant decls *)
+        let defs : list string :=
+          ldef_const_list |> filter (negb ∘ (eq_kername init) ∘ fst)
+                          |> map snd
+                          |> List.app [receive_prelude] (* append const decls after receive prelude decls *)
+                          |> List.app (map snd ldef_ty_list) (* append the above after ty decls*)
+                          in
+          (* map snd (filter (negb ∘ (eq_kername init) ∘ fst) ldef_list) in *)
+        let res : string :=
+            String.concat (nl ++ nl) (defs ++ (cons init_code nil)) in
         inl res
       | None => inr "Error: Empty body for init"
       end
@@ -86,13 +139,14 @@ Definition printCameLIGODefs (prefix : string) (Σ : global_env)
 
 Definition CameLIGO_ignore_default {Base : ChainBase} :=
   [
-    <%% prod %%>
+      <%% prod %%>
     ; <%% @Chain %%>
+    ; <%% @ActionBody %%>
     ; <%% @RecordUpdate.RecordSet.set %%>
     ; <%% @ChainBase %%>
     ; <%% axiomatized_ChainBase %%>
     ; <%% Amount %%>
-    ; <%% Address %%>
+    ; <%% @Address %%>
     ; <%% @address_eqdec %%>
     ; <%% @address_countable %%>
     ; <%% @ContractCallContext %%>
@@ -110,22 +164,8 @@ Definition CameLIGO_call_ctx :=
    (Tezos.amount,
     Tezos.balance)))".
 
-Definition CameLIGO_extract_args := {| 
-  check_wf_env_func := check_wf_env_func extract_within_coq;
-    pcuic_args := {| 
-      dearg_args := Some {| 
-        do_trim_const_masks := true;
-        do_trim_ctor_masks := false; (* cannot have partially applied ctors *)
-        check_closed := true;
-        check_expanded := true;
-        check_valid_masks := true
-      |} 
-    |} 
-  |}.
-
 Definition wrap_in_delimiters s :=
   String.concat nl [""; s].
-
 Definition CameLIGO_extraction {Base : ChainBase} {msg ctx params storage operation : Type}
            (prefix : string)
            (TT_defs : list (kername *  string))
@@ -138,13 +178,14 @@ Definition CameLIGO_extraction {Base : ChainBase} {msg ctx params storage operat
   let TT :=
       (TT_ctors ++ map (fun '(kn,d) => (string_of_kername kn, d)) TT_defs)%list in
   p <- tmEval lazy
-             (printCameLIGODefs prefix Σ TT CameLIGO_extract_args ignore
+             (printCameLIGODefs prefix Σ TT ignore
                                  CameLIGO_call_ctx
                                  m.(lmd_init_prelude)
+                                 m.(lmd_receive_prelude)
                                  init_nm receive_nm) ;;
   match p with
   | inl s =>
     tmEval lazy
-           (wrap_in_delimiters (concat (nl ++ nl) [m.(lmd_prelude); m.(lmd_receive_prelude); s; m.(lmd_entry_point)]))
+           (wrap_in_delimiters (String.concat (nl ++ nl) [m.(lmd_prelude); s; m.(lmd_entry_point)]))
   | inr s => tmFail s
   end.
